policy_proof/coq/security.v
@@ -1,0 +1,23 @@
+Require Import List.
+Require Import Unicode.Utf8.
+
+Require Import query.
+Require Import types.
+
+(* todo *)
+Fixpoint env_ok s (e : env s) : Prop :=
+  match e with
+    | nil => True
+    | (x, t) :: e' =>  False \/ env_ok _ e'
+  end.
+
+(* todo *)
+Theorem secure_query:
+  ∀ s ctx priv e o c,
+    config_ok s ctx priv e =[ o ]=> c →
+      c = config_error \/
+      ∃ s' ctx' priv' e',
+        c = config_ok s' ctx' priv' e' /\ env_ok s' e'.
+Proof.
+  intros.
+Admitted.
