policy_proof/coq/util.v
@@ -1,0 +1,26 @@
+Require Import List.
+Require Import Unicode.Utf8.
+
+Definition hd_option {A : Type} (l : list A) : option A :=
+  match l with
+  | nil => None
+  | cons h _ => Some h
+  end.
+
+Fixpoint eqb_list {A: Type} (eqb: A → A → bool) (l1 l2: list A): bool :=
+  match l1, l2 with
+  | nil, nil => true
+  | nil, _ => false
+  | _, nil => false
+  | h1 :: t1, h2 :: t2 => if eqb h1 h2 then eqb_list eqb t1 t2 else false
+  end.
+
+Theorem eqb_list_refl :
+  ∀ (A : Type) (eqb : A → A → bool),
+    (∀ a, eqb a a = true) → ∀ l, eqb_list eqb l l = true.
+Proof.
+  intros.
+  induction l.
+  - trivial.
+  - simpl.  specialize (H a). rewrite H. apply IHl.
+Qed.
